%!TEX root = ../template.tex
%%%%%%%%%%%%%%%%%%%%%%%%%%%%%%%%%%%%%%%%%%%%%%%%%%%%%%%%%%%%%%%%%%%%
%% annex1.tex
%% NOVA thesis document file
%%
%% Chapter with example of appendix with a short dummy text
%%%%%%%%%%%%%%%%%%%%%%%%%%%%%%%%%%%%%%%%%%%%%%%%%%%%%%%%%%%%%%%%%%%%

\typeout{NT FILE annex2.tex}%


\chapter{Natural Deduction Exercises}
\label{nd-exercises}
In this annex we list all the exercises that were used to evaluate the performance of the algorithm. 
Some of the exercises were collected from the set of practical classes of the \textit{Computational Logic} course at NOVA FCT, 
while others were extracted from a problem pack provided by the University of Oxford, available at:
\url{https://users.ox.ac.uk/~logicman/carr/NDpack.pdf}

\section{Propositional Logic Exercises}
\begin{enumerate}
    \item \(\{\textit{p}, \textit{q}\} \vdash p \land q\)
    \item \(\{\textit{a} \land \textit{b}, \textit{c} \land \textit{d} \land \textit{r}\} \vdash (a \land d) \land r\)
    \item \(\{p \land q\} \vdash q \land p\)
    \item \(\{q \land p, r\} \vdash p \land (r \land q)\)
    \item \(\{a \land b, (c \land d) \land r\} \vdash (a \land d) \land r\)
    \item \(\{p \land (q \land r)\} \vdash (r \land p) \land q\)
    \item \(\vdash p \to p\)
    \item \(\vdash p \to (q \to p)\)
    \item \(\{p \to q, q \to r\} \vdash p \to r\)
    \item \(\vdash p \to ((p \to q) \to q)\)
    \item \(\{(p \to q) \to (p \to r)\} \vdash q \to (p \to r)\)
    \item \(\{(p \to q) \to p\} \vdash q \to p\)
    \item \(\{p \to (q \to r)\} \vdash q \to (p \to r)\)
    \item \(\{p \to (q \to r), p \to q\} \vdash p \to r\)
    \item \(\{p \to p\} \vdash q, (q \to r) \to r\)
    \item \(\vdash (p \to (q \to r)) \to ((p \to q) \to (p \to r))\)
    \item \(\{p \land q\} \vdash p \to q\)
    \item \(\vdash (p \land q) \to p\)
    \item \(\{p \to (q \land r)\} \vdash p \to q\)
    \item \(\{(p \land q) \to q\} \vdash q \to p\)
    \item \(\{(p \land q) \to r\} \vdash p \to (q \to r)\)
    \item \(\{(p \to q) \land (p \to r)\} \vdash p \to (q \land r)\)
    \item \(\{p \to (q \land r)\} \vdash (p \to q) \land (p \to r)\)
    \item \(\{p \lor q\} \vdash q \lor p\)
    \item \(\{p \lor q\} \vdash p \lor (q \lor r)\)
    \item \(\{(p \lor q) \lor r\} \vdash p \lor (q \lor r)\)
    \item \(\{(p \lor q) \lor (r \lor a)\} \vdash (p \lor a) \lor (r \lor q)\)
    \item \(\{p \land (q \lor r)\} \vdash (p \land q) \lor (p \land r)\)
    \item \(\{(p \lor q) \land (p \lor r)\} \vdash p \lor (q \land r)\)
    \item \(\{(p \land q) \lor (p \land r)\} \vdash p \land (q \lor r)\)
    \item \(\{p \lor (q \land r)\} \vdash (p \lor q) \land (p \lor r)\)
    \item \(\{(p \to q) \lor q\} \vdash p \to q\)
    \item \(\{p \lor q\} \vdash (p \to q) \to q\)
    \item \(\{(p \to q) \to (p \to r)\} \vdash (p \lor r) \to (q \to r)\)
    \item \(\{(p \to q) \lor (p \to r)\} \vdash p \to (q \lor r)\)
    \item \(\{(p \to q) \land (q \to p)\} \vdash (p \lor q) \to (p \land q)\)
    \item \(\{(q \to r) \land (q \lor p)\} \vdash (p \to q) \to (r \land q)\)
    \item \(\vdash (p \land q) \to ((p \to q) \to p)\)
    \item \(\{p\} \vdash \lnot \lnot p\)
    \item \(\{\lnot p\} \vdash \lnot(p \land q)\)
    \item \(\{p \to \lnot p\} \vdash \lnot p\)
    \item \(\{\lnot(p \to q)\} \vdash \lnot q\)
    \item \(\{\lnot(p \land q)\} \vdash p \to \lnot q\)
    \item \(\{p \to q\} \vdash \lnot q \to \lnot p\)
    \item \(\vdash \lnot((p \land \lnot p) \lor (q \land \lnot q))\)
    \item \(\{\lnot(p \lor q)\} \vdash \lnot p \land \lnot q\)
    \item \(\{\lnot p \lor \lnot q\} \vdash \lnot(p \land q)\)
    \item \(\{\lnot p\} \vdash p \to q\)
    \item \(\{p \land \lnot p\} \vdash q\)
    \item \(\{p \lor q\} \vdash \lnot p \to q\)
    \item \(\{p \to q, p \land \lnot q\} \vdash r\)
    \item \(\{\lnot \lnot p\} \vdash p\)
    \item \(\vdash p \lor \lnot p\)
    \item \(\{\lnot(\lnot p \lor \lnot q)\} \vdash p \land q\)
    \item \(\{\lnot(p \land q)\} \vdash \lnot p \lor \lnot q\)
    \item \(\{\lnot(p \to q)\} \vdash p\)
    \item \(\{(p \to q) \to p\} \vdash p\)
    \item \(\{(p \to q) \to q\} \vdash \lnot q \to p\)
    \item \(\{\lnot p \land \lnot q\} \vdash \lnot(p \lor q)\)
    \item \(\vdash p \lor (p \to q)\)
    \item \(\vdash (p \to q) \lor (q \to r)\)
    \item \(\{\lnot p \to q, r \lor \lnot q, p \to (a \lor b), \lnot r \land \lnot b\} \vdash a\)
    \item \(\{p \to (q \lor r)\} \vdash (p \to q) \lor (p \to r)\)
    \item \(\vdash a \to (a \lor b)\)
    \item \(\vdash (a \lor a) \to a\)
    \item \(\vdash (a \land b) \to a\)
    \item \(\vdash a \to (b \to a)\)
    \item \(\vdash ((a \to b) \land (b \to c)) \to (a \to c)\)
    \item \(\vdash (a \to (b \to c)) \to ((a \to b) \to (a \to c))\)
    \item \(\vdash (a \to b) \to (a \to (b \lor c))\)
    \item \(\vdash (b \to c) \to ((a \land b) \to c)\)
    \item \(\vdash \lnot(a \lor b) \to \lnot a\)
    \item \(\vdash (b \to c) \to ((a \land b) \to (a \land c))\)
    \item \(\vdash \lnot a \to (a \to b)\)
    \item \(\vdash ((a \to b) \land \lnot b) \to \lnot a\)
    \item \(\vdash (a \to \lnot \lnot a) \land (\lnot \lnot a \to a)\)
    \item \(\vdash ((a \to b) \to (\lnot b \to \lnot a)) \land ((\lnot b \to \lnot a) \to (a \to b))\)
    \item \(\vdash \bot \to a\)
    \item \(\vdash a \lor \lnot a\)
    \item \(\vdash ((a \to d) \to a) \to a\)
    \item \(\vdash a \lor (a \to b)\)
    \item \(\vdash (a \to b) \lor (b \to d)\)
    \item \(\{\lnot a \lor b\} \vdash a \to b\)
    \item \(\{\lnot(a \land b)\} \vdash \lnot a \lor \lnot b\)
    \item \(\{\lnot(a \lor b)\} \vdash \lnot a \land \lnot b\)
    \item \(\{a \lor (b \land c)\} \vdash (a \lor b) \land (a \lor c)\)
    \item \(\{a \land (b \lor c)\} \vdash (a \land b) \lor (a \land c)\)
    \item \(\{(a \to b) \land (b \to a)\} \vdash ((a \land c) \to (b \land c)) \land ((b \land c) \to (a \land c))\)
    \item \(\{\lnot(\lnot a \lor \lnot b)\} \vdash a \land b\)
    \item \(\vdash ((a \to a) \land (a \to a)) \land ((a \to a) \land (a \to a))\)
    \item \(\{p \land q\} \vdash (r \lor s), (p \to r) \lor (q \to s)\)
    \item \(\vdash ((p \to q) \to (\lnot p \lor q)) \land ((\lnot p \lor q) \to (p \to q))\)
    \item \(\vdash (((p \land q) \lor (p \land \lnot q)) \lor (\lnot p \land q)) \lor (\lnot p \land \lnot q)\)
    \item \(\vdash a \to \lnot \lnot a\)
    %\item \(\vdash (((p \to (q \lor s)) \land ((p \land r) \to s)) \land ((s \land t) \to (p \lor \lnot q))) \to (((p \land (q \to r)) \to s) \land (((q \land s) \land t) \to p))\)
    \item \(\vdash ((p \lor q) \lor (r \lor s)) \to ((p \lor s) \lor (r \lor q))\)
    \item \(\{s \lor t, s \to \lnot t, (s \to \lnot t) \to (t \to k)\} \vdash s \lor k\)
    \item \(\vdash (\lnot a \lor \lnot b) \to ((c \to (a \land b)) \to \lnot c)\)
\end{enumerate}

\section{First-Order Logic Exercises}

\begin{enumerate}
    \item \(\{\forall x P(x)\} \vdash \forall y P(y)\)
    \item \(\vdash \forall x (P(x) \rightarrow P(x))\)
    \item \(\{\forall x (P(a) \rightarrow Q(x))\} \vdash P(a) \rightarrow \forall z Q(z)\)
    \item \(\{\forall x P(x) \wedge \forall y Q(y)\} \vdash \forall z (P(z) \wedge Q(z))\)
    \item \(\{\forall x (P(x) \rightarrow Q(x))\} \vdash \forall y_1 P(y_1) \rightarrow \forall y_2 Q(y_2)\)
    \item \(\{\forall z (P(z) \wedge Q(z))\} \vdash \forall y P(y) \wedge \forall y Q(y)\)
    \item \(\{\forall x (P(x) \rightarrow Q(x)), \forall x \neg Q(x)\} \vdash \forall x \neg P(x)\)
    \item \(\{\forall x_1 P(x_1) \vee \forall x_2 Q(x_2)\} \vdash \forall x (P(x) \vee Q(x))\)
    \item \(\{\forall x \forall y (P(x) \rightarrow Q(y))\} \vdash \forall x (P(x) \rightarrow \forall z Q(z))\)
    \item \(\{\forall x (P(x) \rightarrow Q(x)), \forall x (Q(x) \rightarrow R(x))\} \vdash \forall x (P(x) \rightarrow R(x))\)
    \item \(\{\forall x (P(x) \vee Q(x)), \neg \forall x P(x)\} \vdash \neg \forall x \neg Q(x)\)
    \item \(\{\forall x (P(x) \wedge Q(x))\} \vdash \forall x \forall y (P(x) \wedge Q(y))\)
    \item \(\{\forall x \forall y R(x,y)\} \vdash \forall x R(x,x)\)
    \item \(\{\forall x \neg \forall y R(x,y)\} \vdash \neg \forall x \forall y R(x,y)\)
    \item \(\{\forall x R(x,x)\} \vdash \forall x \neg \forall y \neg R(x,y)\)
    \item \(\{\forall x \neg R(x,x)\} \vdash \neg \forall x \forall y (R(x,y) \vee R(y,x))\)
    \item \(\{\neg \forall x \neg \forall y R(y,x)\} \vdash \forall x \neg \forall y \neg R(x,y)\)
    \item \(\{\forall x R(x,x)\} \vdash \forall x \forall y (R(x,y) \rightarrow \neg \forall z \neg (R(x,z) \wedge R(z,y)))\)
    \item \(\{\forall x \forall y R(x,y)\} \vdash \forall x (R(x,x) \wedge \forall y R(y,x))\)
    \item \(\{\forall x \forall y R(x,y)\} \vdash \forall x \forall y (R(x,y) \wedge R(y,x))\)
    \item \(\{\forall x \forall y (R(x,y) \rightarrow R(y,x)), \forall x \forall y \neg (R(x,y) \wedge R(y,x))\} \vdash \forall x \forall y \neg R(x,y)\)
    \item \(\{\forall x \forall y (Q(x,y) \rightarrow Q(y,x)), \forall x \forall y (\neg Q(x,y) \vee \neg Q(y,x))\} \vdash \forall x \forall y \neg Q(x,y)\)
    \item \(\{\forall x \neg R(x,x), \forall x \forall y \forall z ((R(x,y) \wedge R(y,z)) \rightarrow R(x,z))\} \vdash \forall x \forall y \forall z \neg ((R(x,y) \wedge R(y,z)) \wedge R(z,x))\)
    \item \(\{\forall x \forall y \forall z ((R(x,y) \wedge R(x,z)) \rightarrow R(y,z)), \forall x R(x,x)\} \vdash \forall x \forall y \forall z ((R(x,y) \wedge R(y,z)) \rightarrow R(x,z))\)
    \item \(\{\exists x P(x)\} \vdash \exists y P(y)\)
    \item \(\{\neg \exists x P(x)\} \vdash \exists x \neg P(x)\)
    \item \(\{\exists x_1 (P(a) \rightarrow Q(x_1))\} \vdash P(a) \rightarrow \exists x_2 Q(x_2)\)
    \item \(\{\exists x (P(x) \wedge Q(x))\} \vdash \exists y P(y) \wedge \exists z Q(z)\)
    \item \(\{\exists x (P(x) \vee Q(x))\} \vdash \exists y P(y) \vee \exists z Q(z)\)
    \item \(\{\exists x P(x) \vee \exists y Q(y)\} \vdash \exists z (P(z) \vee Q(z))\)
    \item \(\{P(a) \rightarrow \exists x Q(x)\} \vdash \exists x (P(a) \rightarrow Q(x))\)
    \item \(\vdash \exists x \exists y (R(x,y) \rightarrow R(y,x))\)
    \item \(\{\exists x \exists y R(x,y)\} \vdash \exists x \exists y R(y,x)\)
    \item \(\{\exists x R(x,x)\} \vdash \exists x \exists y (R(x,y) \wedge R(y,x))\)
    \item \(\{\neg \exists x \exists y R(x,y)\} \vdash \neg \exists y R(y,y)\)
    \item \(\vdash \neg \exists x \exists y (R(x,y) \wedge \neg R(x,y))\)
    \item \(\vdash \exists x R(x,x) \vee \exists x (R(x,x) \rightarrow \neg \exists y R(y,x))\)
    \item \(\{R(a,b) \wedge R(b,c), \neg Q(a), Q(c)\} \vdash \exists x \exists y ((\neg Q(x) \wedge Q(y)) \wedge R(x,y))\)
    \item \(\{\neg \exists x P(x)\} \vdash \forall x \neg P(x)\)
    \item \(\{\exists x \neg P(x)\} \vdash \neg \forall x P(x)\)
    \item \(\{\neg \forall x P(x)\} \vdash \exists x \neg P(x)\)
    \item \(\{\forall x \neg P(x)\} \vdash \neg \exists x P(x)\)
    \item \(\{\forall x (\exists y P(y) \rightarrow Q(x))\} \vdash \forall x \exists y (P(y) \rightarrow Q(x))\)
    \item \(\{\forall x \neg \forall y (P(x,y) \rightarrow Q(x,y))\} \vdash \forall x \exists y P(x,y)\)
    \item \(\{\forall x (P(x,x) \vee \forall y Q(x,y))\} \vdash \forall x (\exists y P(x,y) \vee Q(x,x))\)
    \item \(\{\exists x (P(x,x) \wedge \forall y Q(x,y))\} \vdash \exists x (\exists y P(x,y) \wedge Q(x,x))\)
    \item \(\vdash \forall x \exists y R(x,y) \vee \neg \forall x R(x,x)\)
    \item \(\{\forall x \exists y R(x,y) \rightarrow \neg \exists x R(x,x), \exists x \forall y R(y,x)\} \vdash \forall x \neg R(x,x)\)
    \item \(\{\forall x (P(x) \rightarrow \exists y R(y,x))\} \vdash \exists z R(z,a) \vee \neg \forall x P(x)\)
    \item \(\{\forall x P(x) \vee \forall x Q(x)\} \vdash \forall x (P(x) \vee Q(x))\)
    \item \(\{\forall x (P(x) \wedge Q(x))\} \vdash \forall x P(x) \wedge \forall x Q(x)\)
    \item \((\vdash \forall x P(x) \wedge \forall x Q(x)) \rightarrow \forall x (P(x) \wedge Q(x))\)
    \item \(\{\exists x (P(x) \wedge Q(x))\} \vdash \exists x P(x) \wedge \exists x Q(x)\)
    \item \((\vdash \exists x P(x) \vee \exists x Q(x)) \rightarrow \exists x (P(x) \vee Q(x))\)
    \item \(\{\exists x (P(x) \vee Q(x))\} \vdash \exists x P(x) \vee \exists x Q(x)\)
    \item \(\{\forall x (P(x) \rightarrow Q(x))\} \vdash \forall x P(x) \rightarrow \forall x Q(x)\)
    \item \(\{\exists y \forall x \phi\} \vdash \forall x \exists y \phi\)
    \item \(\vdash \exists x \neg P(x) \rightarrow \neg \forall x P(x)\)
    \item \(\vdash \neg \forall x P(x) \rightarrow \exists x \neg P(x)\)
    \item \(\vdash \forall x \neg P(x) \rightarrow \neg \exists x P(x)\)
    \item \(\vdash \neg \exists x P(x) \rightarrow \forall x \neg P(x)\)
    \item \(\vdash \exists x \phi \rightarrow \neg \forall x \neg \phi\)
    \item \(\{\neg \forall x \neg \phi\} \vdash \exists x \phi\)
    \item \(\vdash \forall x \phi \rightarrow \neg \exists x \neg \phi\)
    \item \(\{\forall x (C(x) \rightarrow S(x)), \forall x (\neg A(x,b) \rightarrow \neg S(x))\} \vdash \forall x ((C(x) \vee S(x)) \rightarrow A(x,b))\)
    \item \(\{L(a,b), \forall x (\exists y (L(y,x) \vee L(x,y)) \rightarrow L(x,x))\} \vdash \exists x L(x,a)\)
    \item \(\{\forall x \forall y (L(x,y) \rightarrow L(y,x)), \exists x \forall y L(x,y)\} \vdash \forall x \exists y L(x,y)\)
\end{enumerate}

